examples/low-level/MD5.fst
@@ -2,7 +2,7 @@
     options:--admit_fsi Set --z3timeout 10;
     variables:LIB=../../lib;
     other-files:$LIB/ext.fst $LIB/set.fsi $LIB/heap.fst $LIB/st.fst $LIB/list.fst  stack.fst listset.fst
-    st3.fst $LIB/constr.fst word.fst mvector.fsi mvector.fst
+    st3.fst $LIB/constr.fst word.fst mvector.fsi mvector.fst array.fsi array.fst MD5Common.fst
   --*)
 
 (*Why is MD5 so? Why did its designer(s) think
@@ -15,177 +15,47 @@ open MVector
 open Heap
 open Set
 open MachineWord
+open Array
+open MD5Common
 
-(*http://rosettacode.org/wiki/MD5/Implementation#Haskell
- While the version in Haskell and other higher order languages
-is elegant, they do not seem to be memory efficient.
-For example, mapping 64-way in parallel is unnceccesary and we need
-only 4 accumulators at any given time
-*)
-
-val funF : word -> word -> word -> Tot word
-let funF x y z = bitwiseOr (bitwiseAnd x y) (bitwiseAnd (complement x)  z)
-
-(*should these functions also implemented in imperative style?*)
-val funG : word -> word -> word -> Tot word
-let funG x y z = bitwiseOr (bitwiseAnd x z) (bitwiseAnd (complement z)  y)
-
-val funH : word -> word -> word -> Tot word
-let funH x y z =  bitwiseXOR (bitwiseXOR x y) z
-
-val funI : word -> word -> word -> Tot word
-let funI x y z =  bitwiseXOR y (bitwiseAnd (complement z) x)
-
-
-val idxF  : n:nat{n<64} -> Tot (n:nat{n<16})
-let idxF x = x % 16
-
-val idxG  : n:nat{n<64} -> Tot (n:nat{n<16})
-let idxG i = (5 * i + 1) % 16
-
-val idxH  : n:nat{n<64} -> Tot (n:nat{n<16})
-let idxH i = (3 * i + 5) % 16
-
-val idxI  : n:nat{n<64} -> Tot (n:nat{n<16})
-let idxI i = (7 * i) % 16
-
-
-val  funFGHI : n:nat{n<64} -> word -> word -> word -> Tot word
-let funFGHI n =
-  match (n / 16) with
-  | 0 -> (assert (n<16)); funF
-  | 1 -> (assert (16<=n/\n<32)); funG
-  | 2 -> (assert (32<=n/\n<48)); funH
-  | 3 -> (assert (48<=n/\n<64)); funI
-
-
-val  idx : n:nat{n<64} -> n:nat{n<64} -> Tot (n:nat{n<16})
-let idx n =
-  match (n / 16) with
-  | 0 -> (assert (n<16)); idxF
-  | 1 -> (assert (16<=n/\n<32)); idxG
-  | 2 -> (assert (32<=n/\n<48)); idxH
-  | 3 -> (assert (48<=n/\n<64)); idxI
-
-
-
-let rotValues : l:(list (n:nat{n<32}))
-(*{List.length l=16} BUG?*)
- =
-
-[7; 12; 17; 22;     5; 9; 14; 20;    4; 11; 16; 23;    6; 10; 15; 21]
-
-(*#set-options "--initial_fuel 0 --max_fuel 1000 --initial_ifuel 0 --max_ifuel 1000"*)
-
-
-val lenthRotValue : unit ->
-  Lemma
-      (requires True)
-      (ensures (List.length rotValues = 16))
-[SMTPat rotValues]
-let lenthRotValue u = (admit ())
-
-
-val nthT : #a:Type -> l:(list a) -> n:nat{n<List.length l} -> Tot a
-let rec nthT l n = match l with
-h::tl -> if n=0 then h else (nthT tl (n-1))
-
-val rots: n:nat{n<64} -> Tot (n:nat{n<32})
-let rots n =
-  let row:(n:nat{n<4}) = n/16 in
-  let col:(n:nat{n<4}) = n%4 in
-  let index:(n:nat{n<16}) = row*4+col in
-  nthT rotValues index
-
-(**
-floor(abs(sin(i + 1)) × (2 pow 32))
-*)
-assume val consts: n:nat{n<64} -> Tot word
-
-
-(*A chunk of 512 bits, or 16 32 bit words.
-  MD5 processes messages as these chunk *)
-
-
-(*How can we make these private to this file
-  and not corrupt the global namespace?*)
-let iA:(n:nat{n<4})=0
-let iB:(n:nat{n<4})=1
-let iC:(n:nat{n<4})=2
-let iD:(n:nat{n<4})=3
-
-opaque type divides  (divisor :nat) (n:nat) =
-exists (k:nat). k*divisor=n
-
-
-val leastMultipleGeq : n:nat -> div:pos -> Tot (m:nat{divides div m /\ m < n+ div /\ n<=m})
-let leastMultipleGeq n div = admit ()
-(*(div - (n % div)) + n*)
-(*(ceil (n/div))*div*)
-
-(*MOVE to mvector.fsi*)
-type prefixEqual  (#a:Type) (#n1:nat) (#n2:nat)
-  (v1: vector a n1) (v2: vector a n1) (p:nat{p <= n1 /\ p<= n2})
-  = forall (n:nat). n<p ==> atIndex v1 n = atIndex v2 n
-
-
-(*size of the messsage after padding. this function will be used to preallocate
-  an array of the right size*)
-val psize : n:nat -> Tot (m:nat{divides 16 m /\ m < n+ 32 /\ n<=m})
-let psize n =
-  let lm = leastMultipleGeq n 16 in
-  if ((lm+1) % 16 < 12) then lm else lm+16
-
-(*we can tradeoff space for time by not copying the whole thing,
-  but allocate only a new array for padding. Perhaps it can also include
-  the leftofer from the last complete chunk.
-   The MD5 main loop will have to be modified to handle this dichotomy
-  of data/chunk location*)
-(*pads the input*)
-
-assume val cloneAndPad : #n:nat
-  -> r:(ref (vector word n))
-  -> rcloned :(ref (vector word (psize n)))
+assume val cloneAndPad :
+  r:(array word)
+  -> rcloned :(array word)
   -> Mem unit
-      (fun m -> refExistsInMem r m /\ refExistsInMem rcloned m)
-      (fun m0 rp m1  -> refExistsInMem r m0 /\ refExistsInMem rcloned m1
-      (*/\ prefixEqual (loopkupRef r m0) (loopkupRef rp m1) n*)
+      (fun m -> refExistsInMem (asRef r) m /\ refExistsInMem (asRef rcloned) m)
+      (fun m0 rp m1  -> refExistsInMem (asRef r) m0 /\ refExistsInMem (asRef rcloned) m1
+          /\ length rcloned = psize (length r)
+          (*/\ MVector.prefixEqual (loopkupRef r m0) (loopkupRef rp m1) (length r)*)
         )
         (empty)
 
-(*type chunk512 =  vector word 16*)
 
-(**perhaps we should use vector (ref word) n instead of ref (vector word n).
-  Note that it is easy do define subobjects for that style.
-  As a general principle. do we only create refs for words?
- *)
 val processChunk :
-  n : nat
- -> ch:(ref (vector word n))
- -> offset:nat{offset + 16 <= n}
--> acc:(ref (vector word 4))
+ ch:(array word)
+ -> offset:nat{offset + 16 <= (length ch)}
+ -> acc:(array word){length acc=4}
 -> WNSC unit
-    (fun m -> refExistsInMem ch m
-              /\ refExistsInMem acc m /\ ch =!= acc
+    (fun m -> refExistsInMem (asRef ch) m
+              /\ refExistsInMem (asRef acc) m /\ ch =!= acc
               )
-    (fun m0 _ m1 -> refExistsInMem ch m1
-              /\ refExistsInMem acc m1 /\ ch =!= acc
+    (fun m0 _ m1 -> refExistsInMem (asRef ch) m1
+              /\ refExistsInMem (asRef acc) m1 /\ ch =!= acc
               (*/\ loopkupRef  ch m0 = loopkupRef ch m1*)
               )
-    (singleton (Ref acc))
+    (singleton (Ref (asRef acc)))
 
 
-let processChunk n ch offset acc =
+let processChunk ch offset acc =
   let li = salloc #nat 0 in
   scopedWhile1
     li
     (fun liv -> liv < 64)
     (fun m -> True
-              /\ refExistsInMem ch m
-              /\ refExistsInMem acc m
+              /\ refExistsInMem (asRef ch) m
+              /\ refExistsInMem (asRef acc) m
               /\ refExistsInMem li m /\ loopkupRef li m < 65
               )
-    (union (singleton (Ref li)) (singleton (Ref acc)))
+    (union (singleton (Ref li)) (singleton (Ref (asRef acc))))
     (*allRefs ; why does this not work?*)
     (fun u ->
       let liv = memread li in
@@ -195,63 +65,59 @@ let processChunk n ch offset acc =
       let vD = readIndex acc iD in
       let fF:word = funFGHI liv vB vC vD in
       let g:(n:nat{n<16}) = idx liv liv in
-      updIndex acc iD vC;
-      updIndex acc iA vD;
+      writeIndex acc iD vC;
+      writeIndex acc iA vD;
       let mg = readIndex ch (offset+g) in
       let vBr = wmodAdd vA  (wmodAdd fF ( wmodAdd(consts liv)  mg)) in
-      updIndex acc iB (wmodAdd vB (leftrotate (rots liv) vBr));
+      writeIndex acc iB (wmodAdd vB (leftrotate (rots liv) vBr));
       memwrite li (liv+1))
 
-
-assume val initAcc : (vector word 4)
-
 val mainLoop :
-  n : nat{divides 16 n}
- -> ch:(ref (vector word n))
+ ch:(array word){divides 16 (length ch)}
  -> un:unit
  -> WNSC (vector word 4)
-    (fun m -> True /\ refExistsInMem ch m)
-    (fun m0 _ m1 -> True /\ refExistsInMem ch m1)
+    (fun m -> True /\ refExistsInMem (asRef ch) m)
+    (fun m0 _ m1 -> True /\ refExistsInMem (asRef ch) m1)
     (empty)
 
-let mainLoop n ch u =
+let mainLoop ch u =
   let offset = salloc #nat 0 in
-  let acc =  salloc initAcc in
+  let acc =  screateArray initAcc in
   scopedWhile1
     offset
-    (fun offsetv -> offsetv +16 <= n)
+    (fun offsetv -> offsetv +16 <= (length ch))
     (fun m -> True
-              /\ refExistsInMem ch m
-              /\ refExistsInMem acc m
+              /\ refExistsInMem (asRef ch) m
+              /\ refExistsInMem (asRef acc) m
               /\ refExistsInMem offset m
               )
-    (union (singleton (Ref offset)) (singleton (Ref acc)))
+    (union (singleton (Ref offset)) (singleton (Ref (asRef acc))))
     (fun u ->
         let offsetv = memread offset in
-        processChunk n ch offsetv acc;
+        processChunk ch offsetv acc;
         memwrite offset (offsetv + 16));
-  memread acc
+  readArray acc
 
 assume val allZeros : n:nat -> Tot (vector word n)
 
 
 val mD5 : n:nat
- -> ch:(ref (vector word n))
+ -> ch:(array word)
  -> WNSC (vector word 4)
-    (fun m -> True /\ refExistsInMem ch m)
-    (fun m0 _ m1 -> True /\ refExistsInMem ch m1)
+    (fun m -> True /\ refExistsInMem (asRef ch) m)
+    (fun m0 _ m1 -> True /\ refExistsInMem (asRef ch) m1)
     (empty)
 
 let mD5 n ch =
-  let clonedCh = salloc (allZeros (psize n)) in
+  let clonedCh = screateArray (allZeros (psize n)) in
   cloneAndPad ch clonedCh;
   (*withNewScope #(vector word 4)
     #(fun m -> True /\ refExistsInMem ch m)
     #(fun m0 _ m1 -> True /\ refExistsInMem ch m1)
     #(empty)*)
     pushStackFrame ();
-    let mdd5:(vector word 4) = mainLoop (psize n) clonedCh () in
-        popStackFrame (); mdd5
+      let mdd5:(vector word 4) = mainLoop clonedCh () in
+    popStackFrame (); mdd5
 
 (*can we run this program and compare it agains standard implementations?
   That at least needs the following:
